LeanSAT/Reflect/BVExpr/BitBlast.lean
@@ -241,6 +241,20 @@ where
                    dsimp at hlaig hraig
                    omega
                ⟩
+
+          | .xor =>
+             match hfinal:AIG.RefStream.zip raig ⟨lhs, rhs, AIG.mkXorCached⟩ with
+             | ⟨finalAig, s⟩ =>
+               ⟨
+                 ⟨finalAig, s⟩,
+                 by
+                   have : finalAig = (AIG.RefStream.zip raig ⟨lhs, rhs, AIG.mkXorCached⟩).aig := by
+                     simp [hfinal]
+                   simp only [this]
+                   apply AIG.LawfulStreamOperator.le_size_of_le_aig_size
+                   dsimp at hlaig hraig
+                   omega
+               ⟩
     | .un op expr =>
       match op with
       | .not =>
@@ -285,31 +299,8 @@ theorem bitblast.go_decl_eq? (aig : AIG BVBit) (expr : BVExpr w)
     . assumption
   | bin lhs op rhs lih rih =>
     -- TODO: Proof dedup
-    cases op with
-    | and =>
-      dsimp [go]
-      rw [Array.getElem?_lt, Array.getElem?_lt]
-      rw [AIG.LawfulStreamOperator.decl_eq]
-      rw [← Array.getElem?_lt, ← Array.getElem?_lt]
-      rw [rih, lih]
-      -- TODO: for some reason my usual omega attempts fail me here
-      . assumption
-      . apply Nat.lt_of_lt_of_le
-        . exact hidx
-        . exact (bitblast.go aig lhs).property
-      . assumption
-      . apply Nat.lt_of_lt_of_le
-        . exact hidx
-        . apply Nat.le_trans
-          . exact (bitblast.go aig lhs).property
-          . exact (go (go aig lhs).1.aig rhs).property
-      . apply AIG.LawfulStreamOperator.lt_size_of_lt_aig_size
-        apply Nat.lt_of_lt_of_le
-        . exact hidx
-        . apply Nat.le_trans
-          . exact (bitblast.go aig lhs).property
-          . exact (go (go aig lhs).1.aig rhs).property
-    | or =>
+    cases op
+    all_goals
       dsimp [go]
       rw [Array.getElem?_lt, Array.getElem?_lt]
       rw [AIG.LawfulStreamOperator.decl_eq]
